<?xml version="1.0" encoding="UTF-8"?>
<rdf:RDF xmlns:rdf="http://www.w3.org/1999/02/22-rdf-syntax-ns#">
  <skos:ConceptScheme xmlns:skos="http://www.w3.org/2004/02/skos/core#" rdf:about="http://inspire.ec.europa.eu/metadata-codelist/QualityOfServiceCriteria">
    <dc:title xmlns:dc="http://purl.org/dc/elements/1.1/" xml:lang="en">Quality of Service criteria code</dc:title>
    <dcterms:issued xmlns:dcterms="http://purl.org/dc/terms/">2022-10-28T14:56:27</dcterms:issued>
    <dcterms:modified xmlns:dcterms="http://purl.org/dc/terms/">2022-10-28T14:56:27</dcterms:modified>
  </skos:ConceptScheme>
  <skos:Concept xmlns:skos="http://www.w3.org/2004/02/skos/core#" rdf:about="http://inspire.ec.europa.eu/metadata-codelist/QualityOfServiceCriteria/availability">
    <skos:prefLabel xml:lang="en">availability</skos:prefLabel>
    <skos:scopeNote xml:lang="en">The percentage of time the service is available.</skos:scopeNote>
    <skos:prefLabel xml:lang="fr">Disponibilité </skos:prefLabel>
    <skos:scopeNote xml:lang="fr">Indique le pourcentage de temps de disponibilité du service.</skos:scopeNote>
    <skos:inScheme rdf:resource="http://inspire.ec.europa.eu/metadata-codelist/QualityOfServiceCriteria" />
  </skos:Concept>
  <skos:Concept xmlns:skos="http://www.w3.org/2004/02/skos/core#" rdf:about="http://inspire.ec.europa.eu/metadata-codelist/QualityOfServiceCriteria/performance">
    <skos:prefLabel xml:lang="en">performance</skos:prefLabel>
    <skos:scopeNote xml:lang="en">How fast a request to the spatial data service can be completed.</skos:scopeNote>
    <skos:prefLabel xml:lang="fr">Performance </skos:prefLabel>
    <skos:scopeNote xml:lang="fr">Indique la vitesse à laquelle une demande adressée au service de données géographiques peut être exécutée.</skos:scopeNote>
    <skos:inScheme rdf:resource="http://inspire.ec.europa.eu/metadata-codelist/QualityOfServiceCriteria" />
  </skos:Concept>
  <skos:Concept xmlns:skos="http://www.w3.org/2004/02/skos/core#" rdf:about="http://inspire.ec.europa.eu/metadata-codelist/QualityOfServiceCriteria/capacity">
    <skos:prefLabel xml:lang="en">capacity</skos:prefLabel>
    <skos:scopeNote xml:lang="en">The maximum number of simultaneous requests that can be completed with the declared performance.</skos:scopeNote>
    <skos:prefLabel xml:lang="fr">Capacité</skos:prefLabel>
    <skos:scopeNote xml:lang="fr">Indique le nombre maximal de demandes simultanées pouvant être exécutées avec la performance déclarée.</skos:scopeNote>
    <skos:inScheme rdf:resource="http://inspire.ec.europa.eu/metadata-codelist/QualityOfServiceCriteria" />
  </skos:Concept>
</rdf:RDF>

